lib/Marshalling/TupleMarshalling.i.dfy
@@ -1,0 +1,9 @@
+include "MarshalledAccessors.i.dfy"
+
+abstract module Tuple2Marshalling refines Marshalling {
+  import FstMarshalling : Marshalling
+  import SndMarshalling : Marshalling
+
+  type UnmarshalledType = (FstMarshalling.UnmarshalledType, SndMarshalling.UnmarshalledType)
+
+}
